## Faktorregel
>[!note]
>$y = k * f(x)$ → $y' = k*f'(x)$
$k$... Konstante
### Bsp.:
1) $y = 2*x$    $y' = 2*1 = 2$ → $k = 2$
2) $y = e^{1+x} = e*e^x$    $y'=e*e^x=e^{1+x}$
3) $y=f(t) = \frac{1}{2t^2} = \frac{t^{-2}}{2} = \frac{1}{2}t^{-2}$     $y'= \frac{-2}{2} * t^{-3} = - t^{-3}$
4) $y = x * ln2$ → $f'(x) = 1 * ln2 = ln2$
5) $y = \sqrt{\frac{3}{2}x} = \sqrt[k]{\frac{3}{2}} * \sqrt{x}$ → $f'(x) = \sqrt{\frac{3}{2}} * \frac{1}{2}* x ^{-\frac{1}{2}}$

## Summenregel
>[!note]
>$y = u(x) ∓ v(x)$ → $y' = u'(x) ∓ v'(x)$
>kurz: $y' = u' + v'$

1) ![[Drawing 2024-11-27 08.35.07.excalidraw | 1000]]
2) ![[Drawing 2024-11-27 08.38.01.excalidraw | 1000]]
3) ![[Drawing 2024-11-27 08.41.16.excalidraw | 1000]]
4) ![[Drawing 2024-11-27 08.43.00.excalidraw | 1000]]
5) ![[Drawing 2024-11-27 08.45.19.excalidraw | 1000]]